Updated theories

thy/Guard.v
@@ -1,8 +1,326 @@
-Import Esub.Type.
+Require Import Esub.Literal Esub.Ty.
+Require Import Coq.Bool.Bool.
+Require Import Coq.Bool.Sumbool.
+Require Import Coq.Lists.List.
+Require Import Coq.Logic.FunctionalExtensionality.
+Require Import Coq.Arith.PeanoNat.
 
-Inductive guard :=
-| GTrue
-| GFalse
-| GNot : guard -> guard
-| GIf : guard -> guard -> guard -> guard.
+Import ListNotations.
 
+Section maps.
+  Variables K V : Type.
+  Hypothesis Keq_dec : forall (x y : K), {x = y} + {x <> y}.
+
+  Definition map := list (K * V).
+
+  Check fold_left.
+  Check fold_right.
+
+  Fixpoint keys (m : map) : list K :=
+    match m with
+    | nil => nil
+    | (k, v) :: ms => k :: (keys ms)
+    end.
+  
+  Fixpoint mem (k : K) (m : map) : bool :=
+    match m with
+    | nil => false
+    | (k', v) :: ms => if Keq_dec k k' then true else mem k ms
+    end.
+
+  Fixpoint find (k : K) (m : map) : option V :=
+    match m with
+    | nil => None
+    | (k', v) :: ms => if Keq_dec k k' then Some v else find k ms
+    end.
+
+  Fixpoint remove (k : K) (m : map) : map :=
+    match m with
+    | nil => nil
+    | (k', v) :: ms =>
+      if Keq_dec k k' then (k', v) :: (remove k ms) else remove k ms
+    end.
+  
+  Fixpoint add (k : K) (v : V) (m : map) : map :=
+    match m with
+    | nil => [(k, v)]
+    | (k', v') :: ms =>
+      if Keq_dec k k' then (k, v) :: ms else (k', v') :: (add k v ms)
+    end.
+
+
+  Definition map_equiv (m n : map) := forall k, find k m = find k n.
+
+  Lemma map_equiv_refl : forall m, map_equiv m m.
+  Proof.
+    unfold map_equiv. auto.
+  Qed.
+  
+  Lemma map_equiv_sym : forall m n, map_equiv m n -> map_equiv n m.
+  Proof.
+    unfold map_equiv. auto.
+  Qed.
+
+  Lemma map_equiv_trans : forall m n o,
+      map_equiv m n -> map_equiv n o -> map_equiv m o.
+  Proof.
+    unfold map_equiv.
+    congruence.
+  Qed.
+End maps.
+
+
+Fixpoint map_values {K A B : Type} (f : A -> B) (xs : map K A) : map K B :=
+  match xs with
+  | [] => []
+  | (k, v) :: xs => (k, f v) :: (map_values f xs)
+  end.
+
+Check find.
+
+Lemma find_map_Some {K A B : Type} :
+  forall f k Keq_dec v m, find K A Keq_dec k m = Some v -> find K B Keq_dec k (map_values f m) = Some (f v).
+  Proof.
+    intros. generalize dependent k. induction m; intros.
+    - inversion H.
+    - destruct a.
+      simpl in H. simpl.
+      destruct Keq_dec.
+      + inversion H. reflexivity.
+      + apply IHm. assumption.
+  Qed.
+
+  Lemma find_map_None {K A B : Type} :
+    forall f k Keq_dec m, find K A Keq_dec k m = None -> find K B Keq_dec k (map_values f m) = None.
+  Proof.
+    intros. generalize dependent k. induction m; intros.
+    - reflexivity.
+    - destruct a.
+      simpl in H. simpl.
+      destruct Keq_dec.
+      + inversion H.
+      + apply IHm in H. assumption.
+  Qed.
+
+Section sets.
+  Variable A : Type.
+
+  Definition set := list A.
+  Definition union := app.
+End sets.
+
+
+Section guards.
+  Variable V : Type.
+  Hypothesis Veq_dec : forall (x y : V), {x = y} + {x <> y}.
+
+  Inductive guard :=
+  | GTrue
+  | GFalse
+  | GNot : guard -> guard
+  | GIf : guard -> guard -> guard -> guard
+  | GTest : V -> ty -> guard
+  | GEq : V -> lit -> guard.
+
+  Definition Rho := map V lit.
+  Definition Rfind := find V lit Veq_dec.
+  Check Rfind.
+
+  Fixpoint guard_denb (g : guard) (R : Rho) : bool :=
+    match g with
+    | GTrue => true
+    | GFalse => false
+    | GNot g => negb (guard_denb g R)
+    | GIf x t f => if (guard_denb x R) then guard_denb t R else guard_denb f R
+    | GTest v t =>
+      match Rfind v R with
+      | Some l =>
+        match pos_sub (ty_of_lit l) t with
+        | Some _ => true
+        | None => false
+        end
+      | None => false
+      end
+    | GEq v l =>
+      match Rfind v R with
+      | Some l' => (if lit_eq_dec l l' then true else false)
+      | None => false
+      end
+    end.
+
+                  
+                                                         
+
+  Lemma if_idem : forall (b : bool), (if b then true else false) = b.
+  Proof.
+    intros b. destruct b; reflexivity.
+  Qed.
+  
+  Lemma guard_if_idempotent : forall g r, guard_denb g r = guard_denb (GIf g GTrue GFalse) r.
+  Proof.
+    intros g r. simpl. symmetry. apply if_idem.
+  Qed.
+
+  Lemma guard_neg_involutive : forall g r, guard_denb g r = guard_denb (GNot (GNot g)) r.
+  Proof.
+    intros g r. simpl.
+    symmetry. apply negb_involutive.
+  Qed.
+
+  Definition Gamma := map V ty.
+  Definition Gfind := find V ty Veq_dec.
+  Definition Gkeys := keys V ty.
+  Definition Gammas := set Gamma.
+  Definition Gunion := union Gamma.
+
+  Fixpoint any {A : Type} (f : A -> bool) (xs : list A) : bool :=
+    match xs with
+    | [] => false
+    | x :: xs => if f x then true else any f xs
+    end.
+
+  Variables x y : lit.
+  Compute bool_of_sumbool (lit_eq_dec x y).
+
+  
+  Fixpoint guard_denb_gamma (g : guard) (G : Gamma) : bool :=
+    match g with
+    | GTrue => true
+    | GFalse => false
+    | GNot g => negb (guard_denb_gamma g G)
+    | GIf x t f =>
+      if (guard_denb_gamma x G) then guard_denb_gamma t G else guard_denb_gamma f G
+    | GTest v t =>
+      match Gfind v G with
+      | Some s =>
+        match pos_sub s t with
+        | Some _ => true
+        | None => false
+        end
+      | None => false
+      end
+    | GEq v l =>
+      match Gfind v G with
+      | Some t =>
+        match lit_of_ty t with
+        | Some ls =>
+          if any (fun l' => if lit_eq_dec l l' then true else false) ls
+          then true else false
+        | None => false
+        end
+      | None => false
+      end
+    end.
+
+  Lemma guard_denb_denb_gamma : forall g R, guard_denb g R = guard_denb_gamma g (map_values ty_of_lit R).
+    intros g. induction g; intros r.
+    - reflexivity.
+    - reflexivity.
+    - simpl. f_equal. apply IHg.
+    - simpl. rewrite -> IHg1. rewrite -> IHg2. rewrite -> IHg3. reflexivity.
+    - simpl.
+      destruct Rfind eqn:Hr.
+      + unfold Gfind. unfold Rfind in Hr.
+        pose proof (@find_map_Some V lit ty ty_of_lit v Veq_dec l r).
+        apply H in Hr. rewrite -> Hr. reflexivity.
+      + unfold Gfind. unfold Rfind in Hr.
+        pose proof (@find_map_None V lit ty ty_of_lit v Veq_dec r).
+        apply H in Hr. rewrite -> Hr. reflexivity.
+    - simpl.
+      destruct Rfind eqn:Hr.
+      + unfold Gfind. unfold Rfind in Hr.
+        pose proof (@find_map_Some V lit ty ty_of_lit v Veq_dec l0 r).
+        apply H in Hr. rewrite -> Hr.
+        pose proof (lit_of_ty_of_lit l0). rewrite -> H0.
+        simpl.
+        repeat rewrite -> if_idem. reflexivity.
+      + unfold Gfind. unfold Rfind in Hr.
+        pose proof (@find_map_None V lit ty ty_of_lit v Veq_dec r).
+        apply H in Hr. rewrite -> Hr. reflexivity.
+  Qed.
+  
+
+  Fixpoint join_keys (ks : list V) (x y : Gamma) :=
+    match ks with
+    | [] => []
+    | k :: ks =>
+      match (Gfind k x, Gfind k y) with
+      | (Some v1, Some v2) => (k, And v1 v2) :: join_keys ks x y
+      | (Some v1, None) => (k, v1) :: join_keys ks x y
+      | (None, Some v2) => (k, v2) :: join_keys ks x y
+      | (None, None) => join_keys ks x y
+      end
+    end.
+
+  Check List.map.
+
+  
+  Fixpoint In (x : V) (xs : list V) : bool :=
+    match xs with
+    | [] => false
+    | x' :: xs => if Veq_dec x x' then true else In x xs
+    end.
+
+  Fixpoint nub (xs : list V) : list V :=
+    match xs with
+    | [] => []
+    | x :: xs => if In x xs then nub xs else x :: (nub xs)
+    end.
+  
+
+  Fixpoint join1 (x : Gamma) (ys : Gammas) : Gammas :=
+    match ys with
+    | [] => []
+    | y :: ys =>
+      let keys := nub ((Gkeys x) ++ (Gkeys y)) in
+      (join_keys keys x y) :: (join1 x ys)
+    end.
+
+  Fixpoint join (xs : Gammas) (ys : Gammas) : Gammas :=
+    match xs with
+    | [] => []
+    | x :: xs => (join1 x ys) ++ (join xs ys)
+    end.
+
+  Definition empty : Gamma := [].
+  
+  Definition singleton (x : V) (t : ty) : Gamma :=
+    add V ty Veq_dec x t empty.
+
+  Fixpoint guard_type (g : guard) : Gammas * Gammas :=
+    match g with
+    | GTrue => ([empty], [])
+    | GFalse => ([], [empty])
+    | GNot g => (snd (guard_type g), fst (guard_type g))
+    | GIf g t f =>
+      let g_type := guard_type g in
+      let t_type := guard_type t in
+      let f_type := guard_type f in
+      (Gunion (join (fst(g_type)) (fst(t_type))) (join (snd(g_type)) (fst(f_type))),
+       Gunion (join (fst(g_type)) (snd(t_type))) (join (snd(g_type)) (snd(f_type))))
+    | GTest v t => ([singleton v t],[singleton v (Not t)])
+    | GEq v l => let t := Singleton (ty_of_lit l) l in ([singleton v t], [singleton v (Not t)])
+    end.
+
+  Lemma foo : forall v l t, ty_of_lit l = t -> guard_denb (GTest v t) [(v, l)] = true.
+  Proof.
+    intros. simpl.
+    destruct Veq_dec eqn:Veq.
+    - rewrite -> H. rewrite -> pos_sub_refl. reflexivity.
+    - contradiction.
+  Qed.
+    
+End guards.
+
+Definition x := 0.
+Definition y := 1.
+Variable s : ty.
+Variable t : ty.
+
+Check GTest.
+  Definition g1 := (GIf nat (GTest nat x s) (GTrue nat) (GTest nat y t)).
+
+  Definition gt1 := fst (guard_type nat Nat.eq_dec g1).
+  Compute gt1.
+  
+  Compute List.map (fun y => y x) gt1.
