thy/Literal.v
@@ -1,0 +1,12 @@
+Inductive lit :=
+| atom
+| boolean
+| integer
+| tupleNil
+| tupleCons : lit -> lit -> lit.
+
+Lemma lit_eq_dec : forall (x y : lit), {x = y} + {x <> y}.
+Proof.
+  decide equality.
+Qed.
+
