thy/Map.v
@@ -1,0 +1,45 @@
+
+Section total.
+  Variables A B : Type.
+  Hypothesis Aeq_dec : forall (x y : A), {x = y} + {x <> y}.
+  
+  Definition tmap := A -> B.
+
+  Definition update_tmap (v : A) (x : B) (m : tmap) : tmap :=
+    fun w => if Aeq_dec v w then x else m w.
+
+  Lemma update_tmap_apply: forall v x m, (update_tmap v x m) v = x.
+  Proof.
+    intros.
+    unfold update_tmap. destruct Aeq_dec; reflexivity || contradiction.
+  Qed.
+End total.
+
+Section partial.
+  Variables A B : Type.
+  Hypothesis Aeq_dec : forall (x y : A), {x = y} + {x <> y}.
+
+  Definition pmap  := tmap A (option B).
+
+  Local Definition update_map' := update_tmap A (option B) Aeq_dec.
+
+  Definition update_pmap (v : A) (x : B) (m : pmap) : pmap :=
+    update_map' v (Some x) m.
+
+  Lemma update_pmap_apply: forall v x m, (update_pmap v x m) v = Some x.
+  Proof.
+    intros.
+    unfold update_pmap.
+    apply update_tmap_apply.
+  Qed.
+  
+  Definition remove_pmap (v : A) (m : pmap) : pmap :=
+    update_map' v None m.
+
+  Lemma remove_pmap_apply: forall v m, (remove_pmap v m) v = None.
+  Proof.
+    intros.
+    unfold remove_pmap.
+    apply update_tmap_apply.
+  Qed.
+End partial.
