thy/Pattern.v
@@ -1,0 +1,47 @@
+Require Import Esub.Literal.
+
+Section patterns.
+  Variables V : Type.
+  Hypothesis Veq_dec : forall (x y : V), {x = y} + {x <> y}.
+
+  Inductive pat :=
+  | PVar : V -> pat
+  | PLit : lit -> pat
+  | PTupleNil : pat
+  | PTupleCons : pat -> pat -> pat.
+
+  Inductive tuple_pat : pat -> Prop :=
+  | tpTupleNil : tuple_pat PTupleNil
+  | tpTupleCons : forall x y, tuple_pat (PTupleCons x y).
+
+  Inductive wf_pat : pat -> Prop :=
+  | wfpVar : forall v, wf_pat (PVar v)
+  | wfpLit : forall l, wf_pat (PLit l)
+  | wfpTupleNil : wf_pat PTupleNil
+  | wfpTupleCons : forall x y,
+      wf_pat x ->
+      wf_pat y ->
+      tuple_pat y ->
+      wf_pat (PTupleCons x y).
+
+  Fixpoint pat_den (p : pat) (l : lit) : bool :=
+    match p with
+    | PVar v => true
+    | PLit l' => if lit_eq_dec l l' then true else false
+    | PTupleNil =>
+      match l with
+      | TupleNil => true
+      | _ => false
+      end
+    | PTupleCons p1 p2 =>
+      match l with
+      | TupleCons l1 l2 => andb (pat_den p1 l1) (pat_den p2 l2)
+      | _ => false
+      end
+    end.
+End patterns.
+             
+
+  
+  
+        
