thy/Ty.v
@@ -1,0 +1,234 @@
+Require Import Esub.Literal.
+Require Import Coq.Lists.List.
+
+Import ListNotations.
+
+Inductive ty : Type :=
+| Any
+| Atom
+| Boolean
+| Number
+| Integer
+| Tuple
+| TupleNil
+| TupleCons : ty -> ty -> ty
+| Singleton : ty -> lit -> ty
+| Not : ty -> ty
+| And : ty -> ty -> ty
+| Or : ty -> ty -> ty.
+
+Lemma tyeq_dec : forall (x y : ty), {x = y} + {x <> y}.
+Proof.
+  decide equality.
+  apply lit_eq_dec.
+Defined.
+
+Fixpoint ty_of_lit (l : lit) : ty :=
+  match l with
+  | atom => Singleton Atom atom
+  | boolean => Singleton Boolean boolean
+  | integer => Singleton Integer integer
+  | tupleNil => TupleNil
+  | tupleCons x y => TupleCons (ty_of_lit x) (ty_of_lit y)
+  end.
+
+Fixpoint pos_sub (s t : ty) : option ty :=
+  match (s,t) with
+  | (s, Any) => Some s
+  | (Boolean, Atom) => Some Atom
+  | (Integer, Number) => Some Integer
+  | (Singleton s v, Singleton t w) =>
+    match pos_sub s t with
+    | Some u => if lit_eq_dec v w then Some (Singleton u v) else None
+    | None => None
+    end
+  | (Singleton s v, t) =>
+    match pos_sub s t with
+    | Some u => Some (Singleton s v)
+    | None => None
+    end
+  | (TupleNil, Tuple) => Some TupleNil
+  | (TupleCons x y, Tuple) => Some (TupleCons x y)
+  | (TupleCons x1 y1, TupleCons x2 y2) =>
+    match (pos_sub x1 x2, pos_sub y1 y2) with
+    | (Some x', Some y') => Some (TupleCons x' y')
+    | _ => None
+    end
+  | (s, t) => if tyeq_dec s t then Some s else None
+  end.
+
+Definition pos_subb (s t : ty) :=
+  match pos_sub s t with
+  | Some _ => true
+  | None => false
+  end.
+
+Fixpoint ty_den (t : ty) (l : lit) : bool :=
+  match t with
+  | Any => true
+  | Atom => pos_subb (ty_of_lit l) Atom
+  | Boolean => pos_subb (ty_of_lit l) Boolean
+  | Number => pos_subb (ty_of_lit l) Number
+  | Integer => pos_subb (ty_of_lit l) Integer
+  | Tuple => pos_subb (ty_of_lit l) Tuple
+  | TupleNil => pos_subb (ty_of_lit l) TupleNil
+  | TupleCons tx ty =>
+    match l with
+    | tupleCons lx ly => andb (ty_den tx lx) (ty_den ty ly)
+    | _ => false
+    end
+  | Singleton t v =>
+    if lit_eq_dec v l then pos_subb (ty_of_lit l) t else false
+  | Not t => negb (ty_den t l)
+  | And x y => andb (ty_den x l) (ty_den y l)
+  | Or x y => orb (ty_den x l) (ty_den y l)
+  end.
+
+           
+    
+
+
+
+Check fold_left.
+
+Fixpoint pairwise {A B C : Type} (f : A -> B -> C) (xs : list A) (ys : list B) : list C :=
+  flat_map (fun x => map (fun y => f x y) ys) xs.
+
+Notation "'TNone'" := (Not Any) (only parsing) : ty_scope.
+Bind Scope ty_scope with ty.
+Delimit Scope ty_scope with ty.
+
+Inductive tuple_ty : ty -> Prop :=
+| ttNil : tuple_ty TupleNil
+| ttCons : forall x y, tuple_ty (TupleCons x y).
+
+Inductive wf_ty : ty -> Prop :=
+| wfAny : wf_ty Any
+| wfAtom : wf_ty Atom
+| wfBoolean : wf_ty Boolean
+| wfNumber : wf_ty Number
+| wfInteger : wf_ty Integer
+| wfTuple : wf_ty Tuple
+| wfTupleNil : wf_ty TupleNil
+| wfTupleCons : forall x y,
+    wf_ty x ->
+    wf_ty y ->
+    tuple_ty y ->
+    wf_ty (TupleCons x y)
+| wfSingleton : forall x l,
+    wf_ty x ->
+    wf_ty (Singleton x l).
+
+Inductive simple_ty : ty -> Prop :=
+| sAny : simple_ty Any
+| sAtom : simple_ty Atom
+| sBoolean : simple_ty Boolean
+| sNumber : simple_ty Number
+| sInteger : simple_ty Integer.
+
+Inductive compound_ty : ty -> Prop :=
+| cTuple : compound_ty Tuple
+| cTupleNil : compound_ty TupleNil
+| cTupleCons : forall x y,
+    pos_ty x ->
+    pos_ty y ->
+    compound_ty (TupleCons x y)
+| cSingleton : forall x l, 
+    simple_ty x ->
+    compound_ty (Singleton x l)
+with pos_ty : ty -> Prop :=
+     | pSimple : forall x, simple_ty x -> pos_ty x
+     | pCompound : forall x, compound_ty x -> pos_ty x.
+
+Inductive neg_ty : ty -> Prop :=
+| nNot : forall x, pos_ty x -> neg_ty (Not x).
+
+Inductive atom_ty : ty -> Prop :=
+| aPos : forall x, pos_ty x -> atom_ty x
+| aNeg : forall x, neg_ty x -> atom_ty x.
+
+
+Hint Constructors simple_ty compound_ty pos_ty neg_ty atom_ty.
+
+
+Lemma ty_of_lit_pos : forall l, pos_ty (ty_of_lit l).
+Proof.
+  induction l; simpl; auto; reflexivity.
+Qed.
+
+
+
+Fixpoint lit_of_ty (t : ty) : option (list lit) :=
+  match t with
+  | Any => None
+  | Atom => None
+  | Boolean => None
+  | Number => None
+  | Integer => None
+  | Tuple => None
+  | TupleNil => Some [tupleNil]
+  | TupleCons x y =>
+    match (lit_of_ty x, lit_of_ty y) with
+    | (Some xs, Some ys) => Some (pairwise (fun x y => tupleCons x y) xs ys)
+    | _ => None
+    end
+  | Singleton t l => Some [l]
+  | Not t => None
+  | _ => None
+  end.
+
+Lemma lit_of_ty_of_lit : forall l, lit_of_ty (ty_of_lit l) = Some [l].
+Proof.
+  intros.
+  induction l.
+  - reflexivity.
+  - reflexivity.
+  - reflexivity.
+  - reflexivity.
+  - simpl. rewrite -> IHl1. rewrite -> IHl2. reflexivity.
+Qed.
+
+ 
+
+Ltac kill t := repeat (destruct t; simpl).
+Ltac decidable := reflexivity || contradiction.
+
+Lemma pos_sub_refl: forall t, pos_sub t t = Some t.
+Proof with decidable.
+  intros.
+  induction t; simpl.
+  all: try ((try kill tyeq_dec); decidable).
+  - rewrite -> IHt1. rewrite -> IHt2. decidable.
+  - rewrite -> IHt. kill lit_eq_dec; decidable.
+Qed.
+
+Fixpoint pos_inter1 (s t : ty) : option ty :=
+  match (s, t) with
+  | (s, Any) => Some Any
+  | (Boolean, Atom) => Some Boolean
+  | (Integer, Number) => Some Integer
+  | (Singleton s v, Singleton t w) =>
+    match pos_inter1 s t with
+    | Some u => if lit_eq_dec v w then Some (Singleton u v) else None
+    | None => None
+    end
+  | (Singleton s v, t) =>
+    match pos_inter1 s  t with
+    | Some u => Some (Singleton s v)
+    | None => None
+    end
+  | (TupleNil, Tuple) => Some TupleNil
+  | (TupleCons x y, Tuple) => Some (TupleCons x y)
+  | (TupleCons x1 y1, TupleCons x2 y2) =>
+    match (pos_inter1 x1 x2, pos_inter1 y1 y2) with
+    | (Some x', Some y') => Some (TupleCons x' y')
+    | _ => None
+    end
+  | (s, t) => if tyeq_dec s t then Some s else None
+  end.
+
+Definition pos_inter (s t : ty) : option ty :=
+  match pos_inter1 s t with
+  | Some u => Some u
+  | None => pos_inter1 t s
+  end.
